end2end/src/End2EndPipeline.v
@@ -1,0 +1,173 @@
+Require Import String.
+Require Import Coq.ZArith.ZArith.
+Require Import coqutil.Z.Lia.
+Require Import Coq.Lists.List. Import ListNotations.
+Require Import Coq.Logic.FunctionalExtensionality.
+Require Import riscv.Spec.Decode.
+Require Import riscv.Utility.Encode.
+Require Import riscv.Utility.Utility.
+Require Import coqutil.Word.LittleEndian.
+Require Import coqutil.Word.Properties.
+Require Import coqutil.Map.Interface.
+Require Import coqutil.Tactics.Tactics.
+Require Import riscv.Spec.Primitives.
+Require Import riscv.Spec.Machine.
+Require riscv.Platform.Memory.
+Require Import riscv.Spec.PseudoInstructions.
+Require Import riscv.Proofs.EncodeBound.
+Require Import riscv.Proofs.DecodeEncode.
+Require Import riscv.Platform.Run.
+Require Import riscv.Utility.MkMachineWidth.
+Require Import riscv.Utility.Monads. Import MonadNotations.
+Require Import riscv.Utility.runsToNonDet.
+Require Import coqutil.Datatypes.PropSet.
+Require Import riscv.Utility.MMIOTrace.
+Require Import riscv.Platform.RiscvMachine.
+Require Import riscv.Platform.MetricRiscvMachine.
+Require Import riscv.Spec.MetricPrimitives.
+Require Import compiler.RunInstruction.
+Require Import compiler.EventLoop.
+Require Import compiler.ForeverSafe.
+Require Import compiler.GoFlatToRiscv.
+Require Import compiler.Simp.
+Require Import processor.KamiRiscv.
+Require Import bedrock2.Syntax bedrock2.Semantics.
+Require Import compiler.PipelineWithRename.
+Require Import compiler.examples.MMIO.
+Require Import compiler.FlatToRiscvDef.
+
+Local Open Scope Z_scope.
+
+
+Instance FlatToRiscvDef_params: FlatToRiscvDef.parameters := {
+  FlatToRiscvDef.W := KamiWordsInst;
+  FlatToRiscvDef.compile_ext_call := compile_ext_call;
+  FlatToRiscvDef.compile_ext_call_length := compile_ext_call_length';
+  FlatToRiscvDef.compile_ext_call_emits_valid := compile_ext_call_emits_valid;
+}.
+
+Section Connect.
+
+  Context {M: Type -> Type} {MM: Monad M}.
+  Context {Registers: map.map Register Utility.word}
+          {Registers_ok: map.ok Registers}
+          {mem: map.map Utility.word Utility.byte}
+          {mem_ok: map.ok mem}
+          {stringname_env : forall T : Type, map.map string T}
+          {stringname_env_ok: forall T, map.ok (stringname_env T)}
+          {RVM: RiscvProgram M Utility.word}
+          {PRParams : PrimitivesParams M MetricRiscvMachine }
+          {NGstate : Type}
+          {NG : NameGen string NGstate}
+          {src2imp : map.map string Register}.
+
+  Instance mmio_params: MMIO.parameters := {
+    byte_ok := KamiWord.word8ok;
+    word_ok := @KamiWord.wordWok _ (or_introl eq_refl);
+  }.
+
+  Instance pipeline_params: PipelineWithRename.Pipeline.parameters := {
+    FlatToRiscvDef_params := FlatToRiscvDef_params;
+    ext_spec := real_ext_spec;
+    ext_guarantee mach := map.undef_on mach.(getMem) isMMIOAddr;
+  }.
+
+  Context {h: @PipelineWithRename.Pipeline.assumptions pipeline_params}.
+
+  Definition KamiMachine: Type := KamiRiscv.KamiMachine.
+
+  Context (instrMemSizeLg: Z) (dataMemSize: nat).
+
+  Definition kamiStep := kamiStep instrMemSizeLg.
+  Definition states_related := @states_related Pipeline.Registers mem instrMemSizeLg dataMemSize.
+
+  Lemma hl_event_determines_ll_event: forall e' e1 e2,
+      events_related e1 e' ->
+      events_related e2 e' ->
+      e1 = e2.
+  Proof.
+    intros. inversion H; inversion H0; subst; simp; congruence.
+  Qed.
+
+  Lemma hl_trace_determines_ll_trace: forall {t' t1 t2},
+      traces_related t1 t' ->
+      traces_related t2 t' ->
+      t1 = t2.
+  Proof.
+    induction t'; intros.
+    - inversion H. inversion H0. reflexivity.
+    - inversion H. inversion H0. subst. f_equal.
+      + eapply hl_event_determines_ll_event; eassumption.
+      + eapply IHt'; eassumption.
+  Qed.
+
+  Lemma split_ll_trace: forall {t2' t1' t},
+      traces_related t (t2' ++ t1') ->
+      exists t1 t2, t = t2 ++ t1 /\ traces_related t1 t1' /\ traces_related t2 t2'.
+  Proof.
+    induction t2'; intros.
+    - exists t, nil. simpl in *. repeat constructor. assumption.
+    - simpl in H. simp. specialize IHt2' with (1 := H4).
+      destruct IHt2' as (t1 & t2 & E & R1 & R2). subst.
+      exists t1. exists (e :: t2). simpl. repeat constructor; assumption.
+  Qed.
+
+  Lemma states_related_to_traces_related: forall m m' t,
+      states_related (m, t) m' -> traces_related t m'.(getLog).
+  Proof. intros. inversion H. simpl. assumption. Qed.
+
+  (* for debugging f_equal *)
+  Lemma cong_app: forall {A B: Type} (f f': A -> B) (a a': A),
+      f = f' ->
+      a = a' ->
+      f a = f' a'.
+  Proof. intros. congruence. Qed.
+
+  (* to tell that we want string names Semantics.params, because there's also
+     Z names Semantics.params lingering around *)
+  Notation strname_sem := (FlattenExpr.mk_Semantics_params
+                             (@Pipeline.FlattenExpr_parameters pipeline_params)).
+
+  Context (prog: @Program strname_sem)
+          (spec: @ProgramSpec strname_sem)
+          (sat: ProgramSatisfiesSpec prog spec)
+          (ml: MemoryLayout).
+
+  Hypothesis (HinstrMemBound: instrMemSizeLg <= width - 2).
+
+  (* will have to be extended with a program logic proof at the top and with the kami refinement
+     proof to the pipelined processor at the bottom: *)
+  Lemma bedrock2Semantics_to_kamiSpecProcessor:
+    forall (goodTrace: list Event -> Prop) (m1 m2: KamiMachine) (t t0: list Event)
+           (m1': MetricRiscvMachine),
+      (* TODO many more hypotheses will be needed *)
+      states_related (m1, t0) m1' ->
+      star kamiStep m1 m2 t ->
+      exists suffix, goodTrace (suffix ++ t ++ t0).
+  Proof.
+    intros.
+    pose proof (pipeline_proofs prog spec sat ml) as P.
+    edestruct P as (Establish & Preserve & Use); clear P; [admit..|].
+    pose proof @kamiMultiStep_sound as Q.
+    specialize Q with (M := M) (m1 := m1) (m2 := m2) (m1' := m1') (t := t) (t0 := t0)
+                      (instrMemSizeLg := instrMemSizeLg).
+    edestruct Q as (m2' & Rel & InvFinal).
+    - eapply HinstrMemBound.
+    - admit.
+    - eapply Preserve.
+    - eassumption.
+    - eassumption.
+    - eapply Establish. admit.
+    - apply states_related_to_traces_related in Rel.
+      edestruct Use as (suffix & G). 1: exact InvFinal.
+
+    (* TODO ?
+    - apply states_related_to_traces_related in Rel.
+      edestruct Use as (suffix & llTrace & Rel' & G). 1: exact InvFinal.
+      apply split_ll_trace in Rel'.
+      destruct Rel' as (llTrace1 & llTrace2 & E & Rel1' & Rel2'). subst.
+      pose proof (hl_trace_determines_ll_trace Rel Rel1'). subst.
+      exists llTrace2. exact G. *)
+  Admitted.
+
+End Connect.
